---
# Standard Functions
<br/>
$$\frac{d}{dx}\ \left[\ c\ \right]\ =\ 0$$
<br/>
<br/>
$$\frac{d}{dx}\ \left[\ cx\ \right]\ =\ c$$
<br/>
<br/>
$$\frac{d}{dx}\ \left[\ x^{c}\ \right]\ =\ cx^{c-1}$$
<br/>
<br/>
$$\frac{d}{dx}\ \left[\ \frac{1}{x^{c}}\ \right]\ =\ -\frac{1}{x^{c+1}}$$
<br/>
<br/>
$$\frac{d}{dx}\ \left[\ c^{x}\ \right]\ =\ c^{x}\ln(c)$$
<br/>
<br/>
$$\frac{d}{dx}\ \left[\ \ln(cx)\ \right]\ =\ \frac{1}{x}$$
<br/>
<br/>
$$\frac{d}{dx}\ \left[\ \log_c(x)\ \right]\ =\ \frac{1}{x\ln(c)}$$
<br/>
<br/>
---
<br/>
# Trig Functions
<br/>
$$\frac{d}{dx}\ \left[\ \sin({u})\ \right]\ =\ \cos({u})*u'$$
<br/>
<br/>
$$\frac{d}{dx}\ \left[\ \cos({u})\ \right]\ =\ -\sin({u})*u'$$
<br/>
<br/>
$$\frac{d}{dx}\ \left[\ \tan({u})\ \right]\ =\ \sec^{2}({u})*u'$$
<br/>
<br/>
$$\frac{d}{dx}\ \left[\ \csc({u})\ \right]\ =\ -\cot({u})\csc({u})*u'$$
<br/>
<br/>
$$\frac{d}{dx}\ \left[\ \sec({u})\ \right]\ =\ \tan({u})\sec({u})*u'$$
<br/>
<br/>
$$\frac{d}{dx}\ \left[\ \cot({u})\ \right]\ =\ -\csc^{2}({u})*u'$$
<br/>
<br/>
---
<br/>
# Inverse Trig Functions
<br/>
$$\frac{d}{dx}\ \left[\ \sin^{-1}({u})\ \right]\ =\ \frac{u'}{\sqrt{1-u^{2}}}$$
<br/>
<br/>
$$\frac{d}{dx}\ \left[\ \cos^{-1}({u})\ \right]\ =\ -\frac{u'}{\sqrt{1-u^{2}}}$$
<br/>
<br/>
$$\frac{d}{dx}\ \left[\ \tan^{-1}({u})\ \right]\ =\ \frac{u'}{u^{2}+1}$$
<br/>
<br/>
$$\frac{d}{dx}\ \left[\ \csc^{-1}({u})\ \right]\ =\ -\frac{u'}{u^{2}\sqrt{1-\frac{1}{u^{2}}}}$$
<br/>
<br/>
$$\frac{d}{dx}\ \left[\ \sec^{-1}({u})\ \right]\ =\ \frac{u'}{u^{2}\sqrt{1-\frac{1}{u^{2}}}}$$
<br/>
<br/>
$$\frac{d}{dx}\ \left[\ \cot^{-1}({u})\ \right]\ =\ -\frac{u'}{u^{2}+1}$$
<br/>
<br/>
---
<br/>
# Rules of Derivations of Functions
<br/>
$$\frac{d}{dx}\ \left[\ f(x)+g(x)\ \right]\ =\ \frac{d}{dx}f(x)+\frac{d}{dx}g(x)$$
<br/>
<br/>
$$\frac{d}{dx}\ \left[\ f(x)*g(x)\ \right]\ =\ f'(x)g(x)+f(x)g'(x)$$
<br/>
<br/>
$$\frac{d}{dx}\ \left[\ \frac{f(x)}{g(x)}\ \right]\ =\ \frac{f'(x)g(x)-f(x)g'(x)}{\left(g(x)\right)^{2}}$$
<br/>
<br/>
$$\frac{d}{dx}\ \left[\ f(g(x))\ \right]\ =\ f'(g(x))*g'(x)$$
<br/>
<br/>
$$\frac{d}{dx}\ \left[\ x^{u}\ \right]\ =\ x^{u-1}\left(u+x\ln({x})u'\right)$$
<br/>
<br/>
$$\frac{d}{dx}\ \left[\ u^{x}\ \right]\ =\ u^{x}\left(\frac{xu'}{u}+\ln({u})\right)$$
<br/>
<br/>
$$\frac{d}{dx}\ \left[\ u^{k}\ \right]\ =\ u^{k-1}\left(ku'+u\ln({u})k'\right)$$
<br/>
<br/>
---
<br/>
# Specific Cases
<br/>
$$\frac{d}{dx}\ \left[\ \sqrt{x}\ \ \right]\ =\ \frac{1}{2\sqrt{x}}$$
<br/>
<br/>
$$\frac{d}{dx}\ \left[\ \ln({\pm\sin({u})})\ \right]\ =\ \cot({u})*u'$$
<br/>
<br/>
$$\frac{d}{dx}\ \left[\ \ln({\pm\cos({u})})\ \right]\ =\ -\tan({u})*u'$$
